Reorganize project such that relations and corresponding lemmas are grouped together

proof_of_soundness/.CoqMakefile.d
@@ -1,18 +1,30 @@
 ConfigVars.vo ConfigVars.glob ConfigVars.v.beautified ConfigVars.required_vo: ConfigVars.v Syntax.vo
 ConfigVars.vio: ConfigVars.v Syntax.vio
 ConfigVars.vos ConfigVars.vok ConfigVars.required_vos: ConfigVars.v Syntax.vos
-EvalRules.vo EvalRules.glob EvalRules.v.beautified EvalRules.required_vo: EvalRules.v ConfigVars.vo Syntax.vo
-EvalRules.vio: EvalRules.v ConfigVars.vio Syntax.vio
-EvalRules.vos EvalRules.vok EvalRules.required_vos: EvalRules.v ConfigVars.vos Syntax.vos
+EvalRules.vo EvalRules.glob EvalRules.v.beautified EvalRules.required_vo: EvalRules.v ConfigVars.vo MapTheorems.vo Syntax.vo
+EvalRules.vio: EvalRules.v ConfigVars.vio MapTheorems.vio Syntax.vio
+EvalRules.vos EvalRules.vok EvalRules.required_vos: EvalRules.v ConfigVars.vos MapTheorems.vos Syntax.vos
 MapTheorems.vo MapTheorems.glob MapTheorems.v.beautified MapTheorems.required_vo: MapTheorems.v ConfigVars.vo
 MapTheorems.vio: MapTheorems.v ConfigVars.vio
 MapTheorems.vos MapTheorems.vok MapTheorems.required_vos: MapTheorems.v ConfigVars.vos
+NoCallsFromFunctionTable.vo NoCallsFromFunctionTable.glob NoCallsFromFunctionTable.v.beautified NoCallsFromFunctionTable.required_vo: NoCallsFromFunctionTable.v ConfigVars.vo EvalRules.vo Syntax.vo MapTheorems.vo
+NoCallsFromFunctionTable.vio: NoCallsFromFunctionTable.v ConfigVars.vio EvalRules.vio Syntax.vio MapTheorems.vio
+NoCallsFromFunctionTable.vos NoCallsFromFunctionTable.vok NoCallsFromFunctionTable.required_vos: NoCallsFromFunctionTable.v ConfigVars.vos EvalRules.vos Syntax.vos MapTheorems.vos
+NoMacroInvocations.vo NoMacroInvocations.glob NoMacroInvocations.v.beautified NoMacroInvocations.required_vo: NoMacroInvocations.v ConfigVars.vo EvalRules.vo MapTheorems.vo NoCallsFromFunctionTable.vo Syntax.vo
+NoMacroInvocations.vio: NoMacroInvocations.v ConfigVars.vio EvalRules.vio MapTheorems.vio NoCallsFromFunctionTable.vio Syntax.vio
+NoMacroInvocations.vos NoMacroInvocations.vok NoMacroInvocations.required_vos: NoMacroInvocations.v ConfigVars.vos EvalRules.vos MapTheorems.vos NoCallsFromFunctionTable.vos Syntax.vos
+NoVarsInEnvironment.vo NoVarsInEnvironment.glob NoVarsInEnvironment.v.beautified NoVarsInEnvironment.required_vo: NoVarsInEnvironment.v ConfigVars.vo EvalRules.vo Syntax.vo
+NoVarsInEnvironment.vio: NoVarsInEnvironment.v ConfigVars.vio EvalRules.vio Syntax.vio
+NoVarsInEnvironment.vos NoVarsInEnvironment.vok NoVarsInEnvironment.required_vos: NoVarsInEnvironment.v ConfigVars.vos EvalRules.vos Syntax.vos
+SideEffects.vo SideEffects.glob SideEffects.v.beautified SideEffects.required_vo: SideEffects.v ConfigVars.vo EvalRules.vo Syntax.vo
+SideEffects.vio: SideEffects.v ConfigVars.vio EvalRules.vio Syntax.vio
+SideEffects.vos SideEffects.vok SideEffects.required_vos: SideEffects.v ConfigVars.vos EvalRules.vos Syntax.vos
 Syntax.vo Syntax.glob Syntax.v.beautified Syntax.required_vo: Syntax.v 
 Syntax.vio: Syntax.v 
 Syntax.vos Syntax.vok Syntax.required_vos: Syntax.v 
-Theorems.vo Theorems.glob Theorems.v.beautified Theorems.required_vo: Theorems.v Syntax.vo ConfigVars.vo MapTheorems.vo EvalRules.vo Transformations.vo
-Theorems.vio: Theorems.v Syntax.vio ConfigVars.vio MapTheorems.vio EvalRules.vio Transformations.vio
-Theorems.vos Theorems.vok Theorems.required_vos: Theorems.v Syntax.vos ConfigVars.vos MapTheorems.vos EvalRules.vos Transformations.vos
-Transformations.vo Transformations.glob Transformations.v.beautified Transformations.required_vo: Transformations.v Syntax.vo ConfigVars.vo EvalRules.vo
-Transformations.vio: Transformations.v Syntax.vio ConfigVars.vio EvalRules.vio
-Transformations.vos Transformations.vok Transformations.required_vos: Transformations.v Syntax.vos ConfigVars.vos EvalRules.vos
+Theorems.vo Theorems.glob Theorems.v.beautified Theorems.required_vo: Theorems.v Syntax.vo ConfigVars.vo MapTheorems.vo EvalRules.vo SideEffects.vo NoCallsFromFunctionTable.vo NoMacroInvocations.vo NoVarsInEnvironment.vo Transformations.vo
+Theorems.vio: Theorems.v Syntax.vio ConfigVars.vio MapTheorems.vio EvalRules.vio SideEffects.vio NoCallsFromFunctionTable.vio NoMacroInvocations.vio NoVarsInEnvironment.vio Transformations.vio
+Theorems.vos Theorems.vok Theorems.required_vos: Theorems.v Syntax.vos ConfigVars.vos MapTheorems.vos EvalRules.vos SideEffects.vos NoCallsFromFunctionTable.vos NoMacroInvocations.vos NoVarsInEnvironment.vos Transformations.vos
+Transformations.vo Transformations.glob Transformations.v.beautified Transformations.required_vo: Transformations.v Syntax.vo ConfigVars.vo EvalRules.vo SideEffects.vo MapTheorems.vo NoCallsFromFunctionTable.vo NoMacroInvocations.vo NoVarsInEnvironment.vo
+Transformations.vio: Transformations.v Syntax.vio ConfigVars.vio EvalRules.vio SideEffects.vio MapTheorems.vio NoCallsFromFunctionTable.vio NoMacroInvocations.vio NoVarsInEnvironment.vio
+Transformations.vos Transformations.vok Transformations.required_vos: Transformations.v Syntax.vos ConfigVars.vos EvalRules.vos SideEffects.vos MapTheorems.vos NoCallsFromFunctionTable.vos NoMacroInvocations.vos NoVarsInEnvironment.vos
