proof_of_soundness/NoCallsFromFunctionTable.v
@@ -1,0 +1,230 @@
+Require Import
+  Coq.Lists.List
+  Coq.Logic.Classical_Prop.
+
+From Cpp2C Require Import
+  ConfigVars
+  EvalRules
+  Syntax
+  MapTheorems.
+
+
+(* Relation only holds if an expression does not contain any calls from the given
+   function table F' *)
+Inductive ExprNoCallsFromFunctionTable :
+  expr -> function_table -> macro_table -> function_table -> Prop :=
+  | NC_Num : forall z F M F',
+    ExprNoCallsFromFunctionTable (Num z) F M F'
+  | NC_Var : forall x F M F',
+    ExprNoCallsFromFunctionTable (Var x) F M F'
+  | NC_ParenExpr : forall e0 F M F',
+    ExprNoCallsFromFunctionTable e0 F M F' ->
+    ExprNoCallsFromFunctionTable (ParenExpr e0) F M F'
+  | NC_UnExpr : forall uo e0 F M F',
+    ExprNoCallsFromFunctionTable e0 F M F' ->
+    ExprNoCallsFromFunctionTable (UnExpr uo e0) F M F'
+  | NC_BinExpr : forall bo e1 e2 F M F',
+    ExprNoCallsFromFunctionTable e1 F M F' ->
+    ExprNoCallsFromFunctionTable e2 F M F' ->
+    ExprNoCallsFromFunctionTable (BinExpr bo e1 e2) F M F'
+  | NC_Assign : forall x e0 F M F',
+    ExprNoCallsFromFunctionTable e0 F M F' ->
+    ExprNoCallsFromFunctionTable (Assign x e0) F M F'
+  | NC_FunctionCall: forall x es F M F' params fstmt fexpr,
+    ~ StringMap.In x M ->
+    ~ StringMap.In x F' ->
+    ExprNoCallsFromFunctionTableArgs es F M F' ->
+    StringMap.MapsTo x (params, fstmt, fexpr) F ->
+    StmtNoCallsFromFunctionTable fstmt F M F' ->
+    ExprNoCallsFromFunctionTable fexpr F M F' ->
+    ExprNoCallsFromFunctionTable (CallOrInvocation x es) F M F'
+  | NC_MacroInvocation: forall x es F M F' params mexpr ef,
+    ~ StringMap.In x F' ->
+    ExprNoCallsFromFunctionTableArgs es F M F' ->
+    StringMap.MapsTo x (params, mexpr) M ->
+    ExprNoCallsFromFunctionTable mexpr F M F' ->
+    MacroSubst params es mexpr ef ->
+    (* We use (StringMap.remove x M) here because after removing the
+       originally called macro from the macro table (to prevent recursively
+       expanding the macro) we might expose a function from the function table
+       that the macro was shadowing.
+       E.g., say we are checking for a call to the function f in this code:
+
+         #DEFINE f()  f()
+         int f(void) { return 0; }
+
+         int main(void) { return f(); }
+
+       In this case, f is in both the function and macro table.
+       If we searched the original macro table after expanding the
+       macro f for the function f, then we would not find it, because
+       the macro f would still be there shadowing it.
+       In the actual code fragment though, we ultimately would
+       call the function f after expanding the macro f, because the
+       CPP would expand the macro once, not recursively expand it, 
+       and expose the function f to the program. *)
+    ExprNoCallsFromFunctionTable ef F (StringMap.remove x M) F' ->
+    ExprNoCallsFromFunctionTable (CallOrInvocation x es) F M F'
+with ExprNoCallsFromFunctionTableArgs :
+  list expr -> function_table -> macro_table -> function_table -> Prop :=
+  | NC_Args_nil : forall F M F',
+    ExprNoCallsFromFunctionTableArgs nil F M F'
+  | NC_Args_cons : forall e es F M F',
+    ExprNoCallsFromFunctionTable e F M F' ->
+    ExprNoCallsFromFunctionTableArgs es F M F' ->
+    ExprNoCallsFromFunctionTableArgs (e::es) F M F'
+with StmtNoCallsFromFunctionTable :
+  stmt -> function_table -> macro_table -> function_table -> Prop :=
+  | NC_Skip : forall F M F',
+    StmtNoCallsFromFunctionTable Skip F M F'.
+
+
+Lemma ExprNoCallsFromFunctionTable_remove_macro_ExprNoCallsFromFunctionTable :
+  forall e F M F',
+  ExprNoCallsFromFunctionTable e F M F' ->
+  forall x,
+  ExprNoCallsFromFunctionTable e F (StringMap.remove x M) F'.
+Proof.
+  intros e F m F' H. induction H; intros; try constructor; auto.
+  - apply NC_FunctionCall with params fstmt fexpr; auto.
+    + rewrite StringMapFacts.remove_in_iff.
+      (* Issue: Removing a macro from the macro table might expose a function that
+         it shadowed *)
+Abort.
+
+
+Scheme ExprNoCallsFromFunctionTable_mut := Induction for ExprNoCallsFromFunctionTable Sort Prop
+with ExprNoCallsFromFunctionTableArgs_mut := Induction for ExprNoCallsFromFunctionTableArgs Sort Prop
+with StmtNoCallsFromFunctionTable_mut := Induction for StmtNoCallsFromFunctionTable Sort Prop.
+
+
+Lemma EvalExpr_ExprNoCallsFromFunctionTable_remove_function_EvalExpr : forall e F M F',
+  ExprNoCallsFromFunctionTable e F M F' ->
+  forall S E G v S',
+  EvalExpr S E G (StringMapProperties.update F F') M e v S' <->
+  EvalExpr S E G F M e v S'.
+Proof.
+  split.
+  - revert e F M F' H S E G v S'.
+    apply (ExprNoCallsFromFunctionTable_mut
+      (fun e F M F' (h : ExprNoCallsFromFunctionTable e F M F') =>
+        forall S E G v S',
+        EvalExpr S E G (StringMapProperties.update F F') M e v S' ->
+        EvalExpr S E G F M e v S')
+      (fun es F M F' (h : ExprNoCallsFromFunctionTableArgs es F M F') =>
+        forall S E G params vs S' Ef Sargs l,
+        EvalArgs S E G (StringMapProperties.update F F') M params es vs S' Ef Sargs l ->
+        EvalArgs S E G F M params es vs S' Ef Sargs l)
+      (fun stmt F M F' (h : StmtNoCallsFromFunctionTable stmt F M F') =>
+        forall S E G S',
+        EvalStmt S E G (StringMapProperties.update F F') M stmt S' ->
+        EvalStmt S E G F M stmt S')
+      ); intros; try constructor; auto.
+    +
+      inversion_clear H. constructor.
+    +
+      inversion_clear H.
+      * econstructor; eauto.
+      * apply E_GlobalVar with l; auto.
+    +
+      inversion_clear H0; auto.
+    +
+      inversion_clear H0; constructor; auto.
+    +
+      inversion_clear H1. apply E_BinExpr with S'0; auto.
+    +
+      inversion_clear H0.
+      *
+        apply E_Assign_Local with l S'0; auto.
+      *
+        apply E_Assign_Global with l S'0; auto.
+    +
+      inversion_clear H2.
+      *
+        assert ((params, fstmt, fexpr) = (params0, fstmt0, fexpr0)).
+        { apply StringMapFacts.MapsTo_fun with F x; auto.
+          apply StringMapProperties.update_mapsto_iff in H4. destruct H4.
+          + apply StringMap_mapsto_in in H2. contradiction.
+          + apply H2.
+        } inversion H2; subst params0 fstmt0 fexpr0; clear H2.
+        apply E_FunctionCall with
+          params fstmt fexpr ls Ef Sargs S'0 S'' S''' S'''' vs l; auto.
+      *
+        apply StringMap_mapsto_in in H3. contradiction.
+    +
+      inversion_clear H2.
+      *
+        apply StringMap_mapsto_in in m. contradiction.
+      *
+        assert ((params, mexpr) = (params0, mexpr0)).
+        { apply StringMapFacts.MapsTo_fun with M x; auto. }
+        inversion H2; subst params0 mexpr0; clear H2.
+        assert (ef = ef0). { apply MacroSubst_deterministic with params es mexpr; auto. }
+        subst ef0.
+        apply E_MacroInvocation with params mexpr M' ef; subst; auto.
+    +
+      inversion_clear H. constructor.
+    +
+      inversion_clear H1. apply EvalArgs_cons with Snext; auto.
+    +
+      inversion_clear H. constructor.
+  -
+    revert e F M F' H S E G v S'.
+    apply (ExprNoCallsFromFunctionTable_mut
+    (fun e F M F' (h : ExprNoCallsFromFunctionTable e F M F') =>
+      forall S E G v S',
+      EvalExpr S E G F M e v S' ->
+      EvalExpr S E G (StringMapProperties.update F F') M e v S')
+    (fun es F M F' (h : ExprNoCallsFromFunctionTableArgs es F M F') =>
+      forall S E G params vs S' Ef Sargs l,
+      EvalArgs S E G F M params es vs S' Ef Sargs l ->
+      EvalArgs S E G (StringMapProperties.update F F') M params es vs S' Ef Sargs l)
+    (fun stmt F M F' (h : StmtNoCallsFromFunctionTable stmt F M F') =>
+      forall S E G S',
+      EvalStmt S E G F M stmt S' ->
+      EvalStmt S E G (StringMapProperties.update F F') M stmt S')
+    ); intros; try constructor; auto.
+    +
+      inversion_clear H. constructor.
+    +
+      inversion_clear H.
+      * econstructor; eauto.
+      * apply E_GlobalVar with l; auto.
+    +
+      inversion_clear H0; auto.
+    +
+      inversion_clear H0; constructor; auto.
+    +
+      inversion_clear H1. apply E_BinExpr with S'0; auto.
+    +
+      inversion_clear H0.
+      *
+        apply E_Assign_Local with l S'0; auto.
+      *
+        apply E_Assign_Global with l S'0; auto.
+    +
+      inversion_clear H2.
+      *
+        assert ((params, fstmt, fexpr) = (params0, fstmt0, fexpr0)).
+        { apply StringMapFacts.MapsTo_fun with F x; auto. }
+        inversion H2; subst params0 fstmt0 fexpr0; clear H2.
+        apply E_FunctionCall with
+          params fstmt fexpr ls Ef Sargs S'0 S'' S''' S'''' vs l; auto.
+        apply StringMapProperties.update_mapsto_iff. right. auto.
+      *
+        apply StringMap_mapsto_in in H3. contradiction.
+    +
+      inversion_clear H2.
+      *
+        apply StringMap_mapsto_in in m. contradiction.
+      *
+        assert ((params, mexpr) = (params0, mexpr0)).
+        { apply StringMapFacts.MapsTo_fun with M x; auto. }
+        inversion H2; subst params0 mexpr0; clear H2.
+        assert (ef = ef0). { apply MacroSubst_deterministic with params es mexpr; auto. }
+        subst ef0.
+        apply E_MacroInvocation with params mexpr M' ef; subst; auto.
+    + inversion_clear H. constructor.
+    + inversion_clear H1. apply EvalArgs_cons with Snext; auto.
+    + inversion_clear H. constructor.
+Qed.
