proof_of_soundness/NoMacroInvocations.v
@@ -1,0 +1,258 @@
+Require Import
+  Coq.Strings.String.
+
+From Cpp2C Require Import
+  ConfigVars
+  EvalRules
+  MapTheorems
+  NoCallsFromFunctionTable
+  Syntax.
+
+
+Inductive ExprNoMacroInvocations : expr -> function_table -> macro_table -> Prop :=
+  | NM_Num : forall z F M,
+    ExprNoMacroInvocations (Num z) F M
+  | NM_Var : forall x F M,
+    ExprNoMacroInvocations (Var x) F M
+  | NM_ParenExpr : forall e0 F M,
+    ExprNoMacroInvocations e0 F M ->
+    ExprNoMacroInvocations (ParenExpr e0) F M
+  | NM_UnExpr : forall uo e0 F M,
+    ExprNoMacroInvocations e0 F M ->
+    ExprNoMacroInvocations (UnExpr uo e0) F M
+  | NM_Bin_Expr : forall bo e1 e2 F M,
+    ExprNoMacroInvocations e1 F M ->
+    ExprNoMacroInvocations e2 F M ->
+    ExprNoMacroInvocations (BinExpr bo e1 e2) F M
+  | NM_Assign : forall x e0 F M,
+    ExprNoMacroInvocations e0 F M ->
+    ExprNoMacroInvocations (Assign x e0) F M
+  | NM_CallOrInvocation : forall x es F M params fstmt fexpr,
+    ~ StringMap.In x M ->
+    NoMacroInvocationsArgs es F M ->
+    StringMap.MapsTo x (params, fstmt, fexpr) F ->
+    ExprNoMacroInvocations fexpr F M ->
+    ExprNoMacroInvocations (CallOrInvocation x es) F M
+with NoMacroInvocationsArgs : list expr -> function_table -> macro_table -> Prop :=
+  | NM_Args_nil : forall F M,
+    NoMacroInvocationsArgs nil F M
+  | NM_Args_cons : forall e es F M,
+    ExprNoMacroInvocations e F M ->
+    NoMacroInvocationsArgs es F M ->
+    NoMacroInvocationsArgs (e::es) F M.
+
+
+Scheme ExprNoMacroInvocations_mut := Induction for ExprNoMacroInvocations Sort Prop
+with NoMacroInvocationsArgs_mut := Induction for NoMacroInvocationsArgs Sort Prop.
+
+
+Lemma ExprNoMacroInvocations_remove_ExprNoMacroInvocations : forall e F M,
+  ExprNoMacroInvocations e F M ->
+  forall x,
+  ExprNoMacroInvocations e F (StringMap.remove x M).
+Proof.
+  apply (ExprNoMacroInvocations_mut
+    (fun e F M (h : ExprNoMacroInvocations e F M) =>
+      forall x,
+      ExprNoMacroInvocations e F (StringMap.remove x M))
+    (fun es F M (h : NoMacroInvocationsArgs es F M) =>
+      forall x,
+      NoMacroInvocationsArgs es F (StringMap.remove x M))); try constructor; auto.
+  - intros. econstructor; auto.
+    + unfold not. intros. apply StringMapFacts.remove_in_iff in H1. destruct H1.
+      contradiction.
+    + apply m.
+Qed.
+
+
+Lemma ExprNoMacroInvocations_remove_EvalExpr : forall S E G F M e v S',
+  EvalExpr S E G F M e v S' ->
+  ExprNoMacroInvocations e F M ->
+  forall x,
+  EvalExpr S E G F (StringMap.remove x M) e v S'.
+Proof.
+  apply (
+    EvalExpr_mut
+      (* EvalExpr *)
+      (fun S E G F M e v S' (h : EvalExpr S E G F M e v S') =>
+        ExprNoMacroInvocations e F M ->
+        forall x,
+        EvalExpr S E G F (StringMap.remove x M) e v S')
+      (* EvalStmt *)
+      (fun S E G F M stmt S' (h : EvalStmt S E G F M stmt S' ) =>
+        forall (x : string),
+        EvalStmt S E G F (StringMap.remove x M) stmt S' (* TODO: Fix once more statement are added *))
+      (* EvalArgs *)
+      (fun Sprev Ecaller G F M ps es vs Snext Ef Sargs l (h : EvalArgs Sprev Ecaller G F M ps es vs Snext Ef Sargs l) =>
+        NoMacroInvocationsArgs es F M ->
+        forall x,
+        EvalArgs Sprev Ecaller G F (StringMap.remove x M) ps es vs Snext Ef Sargs l )); auto; intros; try constructor.
+  - apply E_LocalVar with l; auto.
+  - apply E_GlobalVar with l; auto.
+  - inversion_clear H0; auto.
+  - inversion_clear H0; auto.
+  - inversion_clear H1. econstructor. auto. auto.
+  - inversion_clear H0. apply E_Assign_Local with l S'; auto.
+  - inversion_clear H0. apply E_Assign_Global with l S'; auto.
+  - inversion_clear H2. apply E_FunctionCall with
+    params fstmt fexpr ls Ef Sargs S' S'' S''' S'''' vs l; auto.
+    + unfold not. intros. apply StringMapFacts.remove_in_iff in H2.
+      destruct H2. contradiction.
+    + apply H1; auto.
+      assert ( (params, fstmt, fexpr) = (params0, fstmt0, fexpr0)).
+      { apply StringMapFacts.MapsTo_fun with F x; auto. }
+      inversion_clear H2. auto.
+  - inversion_clear H0. apply StringMap_mapsto_in in m. contradiction.
+  - inversion_clear H1. econstructor; auto.
+Qed.
+
+
+Lemma ExprNoMacroInvocations_remove_EvalArgs : forall Sprev Ecaller G F M ps es vs Snext Ef Sargs l,
+  EvalArgs Sprev Ecaller G F M ps es vs Snext Ef Sargs l ->
+  NoMacroInvocationsArgs es F M ->
+  forall x,
+  EvalArgs Sprev Ecaller G F (StringMap.remove x M) ps es vs Snext Ef Sargs l.
+Proof.
+  apply (
+    EvalArgs_mut
+      (* EvalExpr *)
+      (fun S E G F M e v S' (h : EvalExpr S E G F M e v S') =>
+        ExprNoMacroInvocations e F M ->
+        forall x,
+        EvalExpr S E G F (StringMap.remove x M) e v S')
+      (* EvalStmt *)
+      (fun S E G F M stmt S' (h : EvalStmt S E G F M stmt S' ) =>
+        forall (x : string),
+        EvalStmt S E G F (StringMap.remove x M) stmt S' (* TODO: Fix once more statement are added *))
+      (* EvalArgs *)
+      (fun Sprev Ecaller G F M ps es vs Snext Ef Sargs l (h : EvalArgs Sprev Ecaller G F M ps es vs Snext Ef Sargs l) =>
+        NoMacroInvocationsArgs es F M ->
+        forall x,
+        EvalArgs Sprev Ecaller G F (StringMap.remove x M) ps es vs Snext Ef Sargs l )); auto; intros; try constructor.
+  - apply E_LocalVar with l; auto.
+  - apply E_GlobalVar with l; auto.
+  - inversion_clear H0; auto.
+  - inversion_clear H0; auto.
+  - inversion_clear H1. econstructor. auto. auto.
+  - inversion_clear H0. apply E_Assign_Local with l S'; auto.
+  - inversion_clear H0. apply E_Assign_Global with l S'; auto.
+  - inversion_clear H2. apply E_FunctionCall with
+    params fstmt fexpr ls Ef Sargs S' S'' S''' S'''' vs l; auto.
+    + unfold not. intros. apply StringMapFacts.remove_in_iff in H2.
+      destruct H2. contradiction.
+    + apply H1; auto.
+      assert ( (params, fstmt, fexpr) = (params0, fstmt0, fexpr0)).
+      { apply StringMapFacts.MapsTo_fun with F x; auto. }
+      inversion_clear H2. auto.
+  - inversion_clear H0. apply StringMap_mapsto_in in m. contradiction.
+  - inversion_clear H1. econstructor; auto.
+Qed.
+
+
+Lemma ExprNoMacroInvocations_update_ExprNoCallFromFunctionTable_ExprNoMacroInvocations :
+  forall e F M,
+  ExprNoMacroInvocations e F M ->
+  forall F',
+  ExprNoCallsFromFunctionTable e F M F' ->
+  ExprNoMacroInvocations e (StringMapProperties.update F F') M.
+Proof.
+  apply (ExprNoMacroInvocations_mut
+    (fun e F M (h : ExprNoMacroInvocations e F M) =>
+      forall F',
+      ExprNoCallsFromFunctionTable e F M F' ->
+      ExprNoMacroInvocations e (StringMapProperties.update F F') M)
+    (fun es F M (h : NoMacroInvocationsArgs es F M) =>
+      forall F',
+      ExprNoCallsFromFunctionTableArgs es F M F' ->
+      NoMacroInvocationsArgs es (StringMapProperties.update F F') M)); intros; try constructor; auto.
+  - inversion_clear H0; auto.
+  - inversion_clear H0; auto.
+  - inversion_clear H1; auto.
+  - inversion_clear H1; auto.
+  - inversion_clear H0; auto.
+  - inversion_clear H1; auto.
+    + assert ((params0, fstmt0, fexpr0) = (params, fstmt, fexpr)).
+      { apply StringMapFacts.MapsTo_fun with F x; auto. }
+      inversion H1; subst params0 fstmt0 fexpr0; clear H1.
+      apply NM_CallOrInvocation with params fstmt fexpr; auto.
+      apply StringMapProperties.update_mapsto_iff. auto.
+    + apply StringMap_mapsto_in in H4. contradiction.
+  - inversion_clear H1; auto.
+  - inversion_clear H1; auto.
+Qed.
+
+
+Lemma ExprNoMacroInvocations_msub_ExprNoMacroInvocations : forall mexpr F M,
+  ExprNoMacroInvocations mexpr F M ->
+  forall e,
+  ExprNoMacroInvocations e F M ->
+  forall p,
+  ExprNoMacroInvocations (msub p e mexpr) F M.
+Proof.
+  intros.
+  induction H; simpl.
+  - constructor.
+  - destruct ((p =? x)%string); auto; constructor.
+  - constructor. auto.
+  - constructor. auto.
+  - constructor. auto. auto.
+  - destruct ( (p =? x)%string ).
+    + destruct e; constructor; apply IHExprNoMacroInvocations; auto.
+    + constructor. apply IHExprNoMacroInvocations; auto.
+  - apply NM_CallOrInvocation with params fstmt fexpr; auto.
+Qed.
+
+
+Lemma ExprNoMacroInvocations_MSub_ExprNoMacroInvocations : forall mexpr F M,
+  ExprNoMacroInvocations mexpr F M ->
+  forall e,
+  ExprNoMacroInvocations e F M ->
+  forall p ef,
+  MSub p e mexpr ef ->
+  ExprNoMacroInvocations ef F M.
+Proof.
+  apply (ExprNoMacroInvocations_mut
+    (fun mexpr F M (h : ExprNoMacroInvocations mexpr F M) =>
+        forall e,
+        ExprNoMacroInvocations e F M ->
+        forall p ef,
+        MSub p e mexpr ef ->
+        ExprNoMacroInvocations ef F M)
+    (fun es F M (h : NoMacroInvocationsArgs es F M) =>
+        forall e,
+        ExprNoMacroInvocations e F M ->
+        forall p es',
+        MSubList p e es es' ->
+        NoMacroInvocationsArgs es' F M)); intros; try (inversion_clear H0; constructor; auto).
+  - inversion H0.
+    + subst. auto.
+    + subst. constructor.
+  - inversion_clear H1. constructor. eapply H. apply H0. apply H2.
+  - inversion_clear H1. constructor. eapply H. apply H0. apply H2.
+  - inversion_clear H2. constructor.
+    + eapply H. apply H1. apply H3.
+    + eapply H0. apply H1. apply H4.
+  - inversion_clear H1.
+    + constructor. apply H with e1 p; auto.
+    + constructor. apply H with e1 p; auto.
+  - inversion_clear H2. apply NM_CallOrInvocation with params fstmt fexpr; auto.
+    apply H with e0 p; auto.
+  - inversion_clear H2. constructor.
+    + apply H with e1 p; auto.
+    + apply H0 with e1 p; auto.
+Qed.
+
+
+Lemma ExprNoMacroInvocations_NoMacroInvocationArgs_MacroSubst_ExprNoMacroInvocations : forall mexpr F M,
+  ExprNoMacroInvocations mexpr F M ->
+  forall es,
+  NoMacroInvocationsArgs es F M ->
+  forall ps ef,
+  MacroSubst ps es mexpr ef ->
+  ExprNoMacroInvocations ef F M.
+Proof.
+  intros. induction H1.
+  - auto.
+  - inversion_clear H0. apply IHMacroSubst; auto.
+    + subst. apply ExprNoMacroInvocations_MSub_ExprNoMacroInvocations with mexpr e p; auto.
+Qed.
