proof_of_soundness/NoVarsInEnvironment.v
@@ -1,0 +1,123 @@
+Require Import
+  Coq.Lists.List
+  Coq.Logic.Classical_Prop
+  Coq.Strings.String.
+
+From Cpp2C Require Import
+  ConfigVars
+  EvalRules
+  Syntax.
+
+
+Inductive ExprNoVarsInEnvironment : expr -> environment -> Prop :=
+  | NV_Num : forall z E,
+    ExprNoVarsInEnvironment (Num z) E
+  | NV_Var : forall x E,
+    ~ StringMap.In x E ->
+    ExprNoVarsInEnvironment (Var x) E
+  | NV_ParenExpr : forall e0 E,
+    ExprNoVarsInEnvironment e0 E ->
+    ExprNoVarsInEnvironment (ParenExpr e0) E
+  | NV_UnExpr : forall uo e0 E,
+    ExprNoVarsInEnvironment e0 E ->
+    ExprNoVarsInEnvironment (UnExpr uo e0) E
+  | NV_Bin_Expr : forall bo e1 e2 E,
+    ExprNoVarsInEnvironment e1 E ->
+    ExprNoVarsInEnvironment e2 E ->
+    ExprNoVarsInEnvironment (BinExpr bo e1 e2) E
+  | NV_Assign : forall x e0 E,
+    ~ StringMap.In x E ->
+    ExprNoVarsInEnvironment e0 E ->
+    ExprNoVarsInEnvironment (Assign x e0) E
+  | NV_CallOrInvocation : forall x es E,
+    ~ StringMap.In x E ->
+    NoVarsInEnvironmentArgs es E ->
+    ExprNoVarsInEnvironment (CallOrInvocation x es) E
+with NoVarsInEnvironmentArgs : list expr -> environment -> Prop :=
+  | NV_Args_nil : forall E,
+    NoVarsInEnvironmentArgs nil E
+  | NV_Args_cons : forall e es E,
+    ExprNoVarsInEnvironment e E ->
+    NoVarsInEnvironmentArgs es E ->
+    NoVarsInEnvironmentArgs (e::es) E.
+
+
+Scheme ExprNoVarsInEnvironment_mut := Induction for ExprNoVarsInEnvironment Sort Prop
+with NoVarsInEnvironmentArgs_mut := Induction for NoVarsInEnvironmentArgs Sort Prop.
+
+
+Lemma ExprNoVarsInEnvironment_msub_ExprNoVarsInEnvironment : forall mexpr E,
+  ExprNoVarsInEnvironment mexpr E ->
+  forall e,
+  ExprNoVarsInEnvironment e E ->
+  forall p,
+  ExprNoVarsInEnvironment (msub p e mexpr) E.
+Proof.
+  intros.
+  induction H; try constructor; try (fold msub; apply IHExprNoVarsInEnvironment; auto).
+  - simpl. destruct ((p =? x)%string); auto. constructor. auto.
+  - fold msub. apply IHExprNoVarsInEnvironment1; auto.
+  - fold msub. apply IHExprNoVarsInEnvironment2; auto.
+  - simpl. destruct ( (p =? x)%string); auto.
+    + destruct e; constructor; auto.
+      inversion_clear H0; auto.
+    + constructor; auto.
+  - auto.
+  - apply H1.
+Qed.
+
+
+Lemma ExprNoVarsInEnvironment_MSub_ExprNoVarsInEnvironment : forall mexpr E,
+  ExprNoVarsInEnvironment mexpr E ->
+  forall e,
+  ExprNoVarsInEnvironment e E ->
+  forall p ef,
+  MSub p e mexpr ef ->
+  ExprNoVarsInEnvironment ef E.
+Proof.
+  apply (ExprNoVarsInEnvironment_mut
+    (fun mexpr E (h : ExprNoVarsInEnvironment mexpr E) =>
+      forall e,
+      ExprNoVarsInEnvironment e E ->
+      forall p ef,
+      MSub p e mexpr ef ->
+      ExprNoVarsInEnvironment ef E)
+    (fun es E (h : NoVarsInEnvironmentArgs es E) =>
+      forall e,
+      ExprNoVarsInEnvironment e E ->
+      forall p es',
+      MSubList p e es es' ->
+      NoVarsInEnvironmentArgs es' E)); intros; try constructor; auto.
+  - inversion_clear H0; constructor.
+  - inversion H0.
+    + subst; auto.
+    + subst. constructor; auto.
+  - inversion_clear H1. constructor. eapply H; eauto.
+  - inversion_clear H1. constructor. eapply H; eauto.
+  - inversion_clear H2. constructor.
+    + eapply H; eauto.
+    + eapply H0; eauto.
+  - inversion H1. 
+    + subst. constructor. inversion H0; auto. eapply H; eauto.
+    + subst. constructor; auto. eapply H; eauto.
+  - inversion_clear H1. constructor; eauto.
+  - inversion_clear H0. constructor.
+  - inversion_clear H2. constructor.
+    + eapply H; eauto.
+    + eapply H0; eauto.
+Qed.
+
+
+Lemma ExprNoVarsInEnvironment_MacroSubst_ExprNoVarsInEnvironment : forall mexpr E,
+  ExprNoVarsInEnvironment mexpr E ->
+  forall es,
+  Forall (fun e => ExprNoVarsInEnvironment e E) es ->
+  forall ps ef,
+  MacroSubst ps es mexpr ef ->
+  ExprNoVarsInEnvironment ef E.
+Proof.
+  intros. induction H1.
+  - auto.
+  - inversion_clear H0. apply IHMacroSubst; auto.
+    apply ExprNoVarsInEnvironment_MSub_ExprNoVarsInEnvironment with mexpr e p; auto.
+Qed.
