proof_of_soundness/SideEffects.v
@@ -1,0 +1,228 @@
+Require Import
+  Coq.Lists.List
+  Coq.Logic.Classical_Prop
+  Coq.Strings.String.
+
+From Cpp2C Require Import
+  ConfigVars
+  EvalRules
+  Syntax.
+
+Fixpoint expr_has_side_effects (e: expr) : bool :=
+  match e with
+  | Num z => false
+  | Var x => false
+  | ParenExpr e0 => expr_has_side_effects e0
+  | UnExpr uo e0 => expr_has_side_effects e0
+  | BinExpr bo e1 e2 =>
+    orb (expr_has_side_effects e1) (expr_has_side_effects e2)
+  (* This is conservative, but matches the behaviour of Clang *)
+  | Assign x e0 => true
+  | CallOrInvocation x es => true
+end.
+
+
+Fixpoint ExprHasSideEffects (e : expr) : Prop :=
+  match e with
+  | Num z => False
+  | Var x => False
+  | ParenExpr e0 => ExprHasSideEffects e0
+  | UnExpr uo e0 => ExprHasSideEffects e0
+  | BinExpr bo e1 e2 =>
+    (ExprHasSideEffects e1) \/ (ExprHasSideEffects e2)
+  (* This is conservative, but matches the behaviour of Clang *)
+  | Assign x e0 => True
+  | CallOrInvocation x es => True
+end.
+
+
+Theorem expr_has_side_effects_ExprHasSideEffects_iff : forall e,
+  expr_has_side_effects e = true <-> ExprHasSideEffects e.
+Proof.
+  split; induction e; intros; simpl in *;
+    try discriminate; try (apply IHe; apply H);
+    try apply I; try contradiction; try reflexivity.
+  - apply Bool.orb_prop in H. tauto.
+  - apply Bool.orb_true_iff. tauto.
+Qed.
+
+
+Theorem expr_side_effects_not_true_not_ExprHasSideEffects_iff : forall e,
+  expr_has_side_effects e <> true <-> ~ ExprHasSideEffects e.
+Proof.
+  split.
+  - intros.
+    rewrite <- expr_has_side_effects_ExprHasSideEffects_iff.
+    unfold not. intros. contradiction.
+  - intros. unfold not. intros.
+    rewrite <- expr_has_side_effects_ExprHasSideEffects_iff in H.
+    contradiction.
+Qed.
+
+
+Lemma not_ExprHasSideEffects_S_Equal : forall e,
+  ~ ExprHasSideEffects e ->
+  forall S E G F M v S',
+  EvalExpr S E G F M e v S' ->
+  NatMap.Equal S S'.
+Proof.
+  intros e H S E G F M v S' E1.
+  induction E1.
+  - reflexivity.
+  - reflexivity.
+  - reflexivity.
+  - apply IHE1. apply H.
+  - apply IHE1. apply H.
+  - unfold ExprHasSideEffects in H. fold ExprHasSideEffects in H.
+    apply Classical_Prop.not_or_and in H.
+    rewrite <- IHE1_1 in IHE1_2.
+    apply IHE1_2.  apply H. apply H.
+  - unfold ExprHasSideEffects in H. contradiction.
+  - unfold ExprHasSideEffects in H. contradiction.
+  - unfold ExprHasSideEffects in H. contradiction.
+  - unfold ExprHasSideEffects in H. contradiction.
+Qed.
+
+
+Lemma not_ExprHasSideEffects_S_eq: forall e,
+  ~ ExprHasSideEffects e ->
+  forall S E G F M v S',
+  EvalExpr S E G F M e v S' ->
+  S = S'.
+Proof.
+  intros e H S E G F M v S' E1.
+  induction E1.
+  - reflexivity.
+  - reflexivity.
+  - reflexivity.
+  - apply IHE1. apply H.
+  - apply IHE1. apply H.
+  - unfold ExprHasSideEffects in H. fold ExprHasSideEffects in H.
+    apply Classical_Prop.not_or_and in H.
+    rewrite <- IHE1_1 in IHE1_2.
+    apply IHE1_2.  apply H. apply H.
+  - unfold ExprHasSideEffects in H. contradiction.
+  - unfold ExprHasSideEffects in H. contradiction.
+  - unfold ExprHasSideEffects in H. contradiction.
+  - unfold ExprHasSideEffects in H. contradiction.
+Qed.
+
+
+Lemma not_ExprHasSideEffects_EvalExpr_EvalExpr : forall e,
+  ~ ExprHasSideEffects e ->
+  forall S E G F M v S',
+  EvalExpr S E G F M e v S' ->
+  EvalExpr S E G F M e v S.
+Proof.
+  intros e H S E G F M v S' E1.
+  induction E1.
+  - apply E_Num.
+  - apply E_LocalVar with l; assumption.
+  - apply E_GlobalVar with l; assumption.
+  - apply E_ParenExpr. apply IHE1. assumption.
+  - apply E_UnExpr. apply IHE1. assumption.
+  - unfold ExprHasSideEffects in H. fold ExprHasSideEffects in H.
+    apply Classical_Prop.not_or_and in H. destruct H. apply E_BinExpr with S'.
+    + assumption.
+    + apply not_ExprHasSideEffects_S_eq in E1_1.
+      * subst. apply IHE1_2. assumption.
+      * assumption.
+  - unfold ExprHasSideEffects in H. contradiction.
+  - unfold ExprHasSideEffects in H. contradiction.
+  - unfold ExprHasSideEffects in H. contradiction.
+  - unfold ExprHasSideEffects in H. contradiction.
+Qed.
+
+
+Theorem Forall_not_ExprHasSideEffects_EvalArgs_S_Equal : forall S E G F M ps es S' vs Ef Sargs l,
+  Forall (fun e => ~ ExprHasSideEffects e ) es ->
+  EvalArgs S E G F M ps es vs S' Ef Sargs l ->
+  NatMap.Equal S S'.
+Proof.
+  intros. induction H0.
+  - reflexivity.
+  - inversion H. apply not_ExprHasSideEffects_S_eq in H0.
+    rewrite H0. apply IHEvalArgs. assumption. assumption.
+Qed.
+
+
+Theorem Forall_not_ExprHasSideEffects_EvalArgs_S_eq : forall S E G F M ps es S' vs Ef Sargs l,
+  Forall (fun e => ~ ExprHasSideEffects e ) es ->
+  EvalArgs S E G F M ps es vs S' Ef Sargs l ->
+  S = S'.
+Proof.
+  intros. induction H0.
+  - reflexivity.
+  - inversion H. apply not_ExprHasSideEffects_S_eq in H0.
+    rewrite H0. apply IHEvalArgs. assumption. assumption.
+Qed.
+
+
+Lemma Forall_not_ExprHasSideEffects_EvalArgs_EvalArgs: forall S E G F M ps es S' vs Ef Sargs l,
+  Forall (fun e => ~ ExprHasSideEffects e ) es ->
+  EvalArgs S E G F M ps es vs S' Ef Sargs l ->
+  EvalArgs S E G F M ps es vs S Ef Sargs l.
+Proof.
+  intros. induction H0.
+  - apply EvalArgs_nil.
+  - inversion H; subst. apply EvalArgs_cons with Snext; auto.
+    + apply not_ExprHasSideEffects_S_eq in H0; subst; auto.
+Qed.
+
+
+Lemma Skip_S_Equal : forall S E G F M S',
+  EvalStmt S E G F M Skip S' ->
+  NatMap.Equal S S'.
+Proof.
+  intros. induction H. reflexivity.
+Qed.
+
+
+Lemma Skip_S_eq : forall S E G F M S',
+  EvalStmt S E G F M Skip S' ->
+  S = S'.
+Proof.
+  intros. induction H. reflexivity.
+Qed.
+
+
+Lemma not_ExprHasSideEffects_msub_not_ExprHasSideEffects : forall mexpr p e,
+  ~ ExprHasSideEffects mexpr ->
+  ~ ExprHasSideEffects e ->
+  ~ ExprHasSideEffects (msub p e mexpr).
+Proof.
+  induction mexpr; auto.
+  - (* Var *)
+    intros. simpl in *. destruct ((p =? x)%string); auto.
+  - (* BinExpr *)
+    intros. simpl in *. apply Classical_Prop.not_or_and in H. destruct H.
+    apply Classical_Prop.and_not_or. split; auto.
+  - (* Assign *)
+    intros. simpl in *. contradiction.
+Qed.
+
+
+Lemma not_ExprHasSideEffects_Msub_not_ExprHasSideEffects : forall p e mexpr ef,
+  ~ ExprHasSideEffects mexpr ->
+  ~ ExprHasSideEffects e ->
+    MSub p e mexpr ef ->
+  ~ ExprHasSideEffects ef.
+Proof.
+  intros. induction H1; auto.
+  simpl in *. apply Classical_Prop.not_or_and in H. destruct H.
+  apply Classical_Prop.and_not_or. auto.
+Qed.
+
+
+Theorem not_ExprHasSideEffects_MacroSubst_not_ExprHasSideEffects : forall mexpr params es ef,
+  ~ ExprHasSideEffects mexpr ->
+  Forall (fun e => ~ ExprHasSideEffects e) es ->
+  MacroSubst params es mexpr ef ->
+  ~ ExprHasSideEffects ef.
+Proof.
+  intros.
+  induction H1; auto.
+  inversion H0; subst.
+  apply IHMacroSubst; eauto using not_ExprHasSideEffects_Msub_not_ExprHasSideEffects.
+Qed.
+
